show that our new execution of loop_inv is a function

backend/PolyIR.v
@@ -1699,19 +1699,56 @@ Abort.
 (* Create a relation that allows one to peel the last iteration off of
 a loop *)
 Inductive exec_loop_inv: loopenv -> mem -> loop -> mem -> loopenv -> Prop :=
-| exec_loop_inv_start: forall (m: mem) (l: loop) (le: loopenv),
-    exec_loop_inv le m l m le
-| exec_loop_inv_last_iter: forall (l: loop) (le le': loopenv) (m mloop mstmt: mem),
-    (viv le < loopub l)%nat ->
-    exec_loop_inv le m l mloop le' ->
-    exec_stmt le' l mloop (loopstmt l) mstmt ->
-    exec_loop_inv le m l mstmt (loopenv_bump_vindvar le')
+| exec_loop_inv_start: forall (m0: mem) (l: loop) (le0: loopenv),
+    (viv le0 < loopub l)%nat ->
+    (viv le0 = 0)%nat ->
+    exec_loop_inv le0 m0 l m0 le0
+| exec_loop_inv_last_iter: forall (l: loop) (le0 le1: loopenv) (m0 m1 m2: mem),
+    (viv le0 < loopub l)%nat ->
+    (viv le0 > 0)%nat ->
+    exec_loop_inv le0 m0 l m1 le1 ->
+    exec_stmt le1 l m1 (loopstmt l) m2 ->
+    exec_loop_inv le0 m0 l m2 (loopenv_bump_vindvar le1)
 | exec_loop_inv_out_of_bounds:
     forall (l: loop) (le: loopenv) (m: mem),
       (viv le >= loopub l)%nat ->
       exec_loop_inv le m l m le.
 
 
+Theorem exec_loop_inv_is_function:
+  forall (le le1: loopenv) (m m1: mem) (l: loop),
+    exec_loop_inv le m l m1 le1 ->
+    forall (le2: loopenv) (m2: mem),
+      exec_loop_inv le m l m2 le2 ->
+      le1 = le2 /\ m1 = m2.
+Proof.
+  intros until l.
+  intros exec1.
+  induction exec1;
+    subst.
+
+  - intros until m2. intros exec2.
+    induction exec2; try omega; try auto.
+  - intros until m3.
+    intros exec2.
+    induction exec2; try auto; try omega.
+    assert ( le1 = le2 /\ m1 = m3) as eqs.
+    apply IHexec1; assumption.
+    destruct eqs as [leq meq].
+    subst.
+
+    assert (m2 = m4) as meq.
+    eapply exec_stmt_is_function;
+      eassumption.
+
+    subst.
+
+    auto.
+
+  -  intros until m2. intros exec2.
+     induction exec2; try omega; try auto.
+Qed.
+  
 
 (* Show how the usual order of execution matches the order of execution
 where we peel the final loop iter off *)
